hocap rand progress

theories/coneris/lib/hocap_rand.v
@@ -105,12 +105,18 @@ Class rand_spec `{!conerisGS Σ} := RandSpec
     (∀ l, length l = num ->  0<= ε2 l)%R ->
     (SeriesC (λ l, if bool_decide (l ∈ enum_uniform_fin_list tb num) then ε2 l else 0) /((S tb)^num) <= ε)%R->
     is_rand (L:=L) N γ1 γ2 -∗
-    (□∀ (ε':R) ns', (P ∗ rand_error_auth (L:=L) γ1 (ε')%R ∗ ⌜length ns' = num⌝) ={E∖↑N}=∗
-                  ∃ diff: R, ⌜(0<=diff)%R⌝ ∗ ⌜(ε' = ε+diff)%R⌝ ∗  
-        (⌜(1<=ε2 ns' + diff)%R⌝ ∨ (rand_error_auth (L:=L) γ1 (ε2 ns' + diff)%R ∗ T ns')))
+    □(∀ (ε': R) m, P ∗rand_error_auth (L:=L) γ1 (ε')%R ∗ rand_tapes_auth (L:=L) γ2 m ={E∖↑N}=∗
+                   ⌜(ε<=ε')%R⌝ ∗ ⌜(m!!α = Some (tb, ns))⌝ ∗
+                   P ∗rand_error_auth (L:=L) γ1 (ε')%R ∗ rand_tapes_auth (L:=L) γ2 m 
+      ) -∗
+    (□∀ (ε':R) ns' m, (P ∗ rand_error_auth (L:=L) γ1 (ε')%R ∗ ⌜length ns' = num⌝ ∗
+                     rand_tapes_auth (L:=L) γ2 m
+                    ) ={E∖↑N}=∗
+                             (⌜(1<=ε2 ns' + (ε'-ε))%R⌝ ∨ (rand_error_auth (L:=L) γ1 (ε2 ns' + (ε'-ε))%R ∗
+                                                       rand_tapes_auth (L:=L) γ2 (<[α:= (tb, ns++(fin_to_nat <$> ns'))]> m) ∗ T ns')))
         -∗
-    P -∗ rand_tapes_frag (L:=L) γ2 α (tb, ns)-∗
-        wp_update E (∃ n, T n ∗ rand_tapes_frag (L:=L) γ2 α (tb, ns++(fin_to_nat <$> n)))
+    P -∗ 
+        wp_update E (∃ n, T n)
 }.
 
 Section impl.
@@ -281,98 +287,359 @@ Section impl.
 Qed.
 Next Obligation.
   simpl.
-  iIntros (??????????????? Hsubset Hpos Hineq) "#Hinv #Hvs HP Hfrag".
+  iIntros (??????????????? Hsubset Hpos Hineq) "#Hinv #Hchange #Hvs HP".
   iApply wp_update_state_step_coupl.
   iIntros (σ1 ε_supply) "((Hheap&Htapes)&Hε)".
   iMod (inv_acc with "Hinv") as "[>(%ε' & % & H1 & H2 & H3 & H4 ) Hclose]"; [done|].
-  iDestruct (hocap_tapes_agree with "[$][$]") as "%K".
+  iMod ("Hchange" with "[$]") as "(%&%&HP & H2 &H4)". 
+  (* iDestruct (hocap_tapes_agree with "[$][$]") as "%K". *)
   iDestruct (big_sepM_insert_acc with "[$]") as "[Htape H3]"; first done.
   simpl.
   iDestruct (tapeN_lookup with "[$][$]") as "(%&%&%Heq)".
   iDestruct (ec_supply_bound with "[$][$]") as "%".
   iMod (ec_supply_decrease with "[$][$]") as (ε'' ε_rem -> Hε') "Hε_supply". subst.
+  iApply fupd_mask_intro; [set_solver|]; iIntros "Hclose'".
+  iApply (state_step_coupl_iterM_state_adv_comp_con_prob_lang num α); first done.
+  unshelve iExists (λ x, mknonnegreal (if length x =? num then ε2 x + (ε''-ε) else 1)%R _).
+  { case_match; last (simpl;lra). admit. }
+  iSplit.
+  { iPureIntro.
+    simpl. admit.
+    (* unshelve epose proof (Hineq ε1' _) as H'; first apply cond_nonneg. *)
+    (* etrans; last exact. *)
+    (* rewrite (Rdiv_def _ (2^_)) -SeriesC_scal_r. *)
+    (* etrans; last eapply (SeriesC_le_inj _ (λ x, Some (nat_to_bool <$> (fin_to_nat <$> x)))). *)
+    (* - apply SeriesC_le. *)
+    (*   + simpl. intros n. *)
+    (*     rewrite !fmap_length. *)
+    (*     case_match. *)
+    (*     * replace (1+1)%R with 2%R by lra. *)
+    (*       rewrite -Rdiv_1_l. simpl. *)
+    (*       split; last lra. *)
+    (*       apply Rmult_le_pos. *)
+    (*       -- apply Rcomplements.Rdiv_le_0_compat; first lra. *)
+    (*          apply pow_lt; lra. *)
+    (*       -- apply Hpos; first done. *)
+    (*          rewrite !fmap_length. *)
+    (*          by apply Nat.eqb_eq. *)
+    (*     * lra. *)
+    (*   + simpl. *)
+    (*     apply (ex_seriesC_list_length _ num). *)
+    (*     intros ?. rewrite !fmap_length. *)
+    (*     case_match; last lra. *)
+    (*     intros. by apply Nat.eqb_eq. *)
+    (* - intros. case_match; last lra. *)
+    (*   apply Rmult_le_pos; first apply Hpos; simpl; auto. *)
+    (*   + by apply Nat.eqb_eq. *)
+    (*   + rewrite -Rdiv_1_l. *)
+    (*     apply Rcomplements.Rdiv_le_0_compat; first lra. *)
+    (*     apply pow_lt; lra. *)
+    (* - intros ??? <- K. *)
+    (*   simplify_eq. *)
+    (*   rewrite -!list_fmap_compose in K. *)
+    (*   apply list_fmap_eq_inj in K; try done. *)
+    (*   intros x x'. *)
+    (*   repeat (inv_fin x; try intros x); *)
+    (*     repeat (inv_fin x'; try intros x'); done. *)
+    (* - apply (ex_seriesC_list_length _ num). *)
+    (*     intros ?. *)
+    (*     case_match; last lra. *)
+    (*     intros. by apply Nat.eqb_eq. *)
+  }
+  iIntros (sample) "<-".
+  destruct (Rlt_decision (nonneg ε_rem + (ε2 sample + (ε''-ε))%R) 1%R) as [Hdec|Hdec]; last first.
+  { apply Rnot_lt_ge, Rge_le in Hdec.
+    iApply state_step_coupl_ret_err_ge_1.
+    simpl. simpl in *. rewrite Nat.eqb_refl. lra.
+  }
+  iApply state_step_coupl_ret.
+  unshelve iMod (ec_supply_increase _ (mknonnegreal (ε2 sample + (ε''-ε))%R _) with "Hε_supply") as "[Hε_supply Hε]".
+  { admit. }
+  { simpl. done. }
+  simpl.
+  iMod (tapeN_update_append' _ _ _ _ sample with "[$][$]") as "[Htapes Htape]".
+  (* iMod (hocap_tapes_update _ _ _ _ _ _ ((fin_to_nat <$> ns')++(fin_to_nat <$> sample)) with "[$][$]") as "[H4 Hfrag]". *)
+  iMod "Hclose'" as "_".
+  iMod ("Hvs" $! ε'' sample  with "[$HP $H2 $H4]") as "[%|(Hauth & H2 & HT)]"; first done.
+  { iExFalso. iApply (ec_contradict with "[$]"). exact. }
+  iMod ("Hclose" with "[$Hε $Hauth Htape H3 $H2]") as "_".
+  { iNext.
+    by iApply "H3".
+  }
+  iApply fupd_mask_intro_subseteq; first set_solver.
+  iFrame. 
+  erewrite (nnreal_ext _ _); first done.
+  simpl. by rewrite Nat.eqb_refl.
 Admitted.
-(*   iApply fupd_mask_intro; [set_solver|]; iIntros "Hclose'". *)
-(*   iApply (state_step_coupl_iterM_state_adv_comp_con_prob_lang num α); first done. *)
-(*   pose (diff := (ε'' - ε)%R). *)
-(*   unshelve iExists (λ x, mknonnegreal (if length x =? num then ε2 x + (diff/ ((S tb) ^ num))else 1)%R _). *)
-(*   { case_match; last (simpl;lra). apply Hpos. by apply Nat.eqb_eq. } *)
-(*   iSplit. *)
-(*   { iPureIntro. *)
-(*     simpl. *)
-(*     unshelve epose proof (Hineq ε1' _) as H'; first apply cond_nonneg. *)
-(*     etrans; last exact. *)
-(*     rewrite (Rdiv_def _ (2^_)) -SeriesC_scal_r. *)
-(*     etrans; last eapply (SeriesC_le_inj _ (λ x, Some (nat_to_bool <$> (fin_to_nat <$> x)))). *)
-(*     - apply SeriesC_le. *)
-(*       + simpl. intros n. *)
-(*         rewrite !fmap_length. *)
-(*         case_match. *)
-(*         * replace (1+1)%R with 2%R by lra. *)
-(*           rewrite -Rdiv_1_l. simpl. *)
-(*           split; last lra. *)
-(*           apply Rmult_le_pos. *)
-(*           -- apply Rcomplements.Rdiv_le_0_compat; first lra. *)
-(*              apply pow_lt; lra. *)
-(*           -- apply Hpos; first done. *)
-(*              rewrite !fmap_length. *)
-(*              by apply Nat.eqb_eq. *)
-(*         * lra. *)
-(*       + simpl. *)
-(*         apply (ex_seriesC_list_length _ num). *)
-(*         intros ?. rewrite !fmap_length. *)
-(*         case_match; last lra. *)
-(*         intros. by apply Nat.eqb_eq. *)
-(*     - intros. case_match; last lra. *)
-(*       apply Rmult_le_pos; first apply Hpos; simpl; auto. *)
-(*       + by apply Nat.eqb_eq. *)
-(*       + rewrite -Rdiv_1_l. *)
-(*         apply Rcomplements.Rdiv_le_0_compat; first lra. *)
-(*         apply pow_lt; lra. *)
-(*     - intros ??? <- K. *)
-(*       simplify_eq. *)
-(*       rewrite -!list_fmap_compose in K. *)
-(*       apply list_fmap_eq_inj in K; try done. *)
-(*       intros x x'. *)
-(*       repeat (inv_fin x; try intros x); *)
-(*         repeat (inv_fin x'; try intros x'); done. *)
-(*     - apply (ex_seriesC_list_length _ num). *)
-(*         intros ?. *)
-(*         case_match; last lra. *)
-(*         intros. by apply Nat.eqb_eq. *)
-(*   } *)
-(*   iIntros (sample) "<-". *)
-(*   destruct (Rlt_decision (nonneg ε_rem + (ε2 ε1' (nat_to_bool <$> (fin_to_nat <$> sample))))%R 1%R) as [Hdec|Hdec]; last first. *)
-(*   { apply Rnot_lt_ge, Rge_le in Hdec. *)
-(*     iApply state_step_coupl_ret_err_ge_1. *)
-(*     simpl. simpl in *. rewrite Nat.eqb_refl. lra. *)
-(*   } *)
-(*   iApply state_step_coupl_ret. *)
-(*   unshelve iMod (ec_supply_increase _ (mknonnegreal (ε2 ε1' (nat_to_bool <$> (fin_to_nat <$> sample))) _) with "Hε_supply") as "[Hε_supply Hε]". *)
-(*   { apply Hpos; first apply cond_nonneg. by rewrite !fmap_length. } *)
-(*   { simpl. done. } *)
-(*   simpl. *)
-(*   iMod (tapeN_update_append' _ _ _ _ sample with "[$][Htape]") as "[Htapes Htape]". *)
-(*   { by erewrite Heq. } *)
-(*   iMod (hocap_tapes_presample' _ _ _ _ _ (fin_to_nat <$> sample) with "[$][$]") as "[H4 Hfrag]". *)
-(*   iMod "Hclose'" as "_". *)
-(*   iMod ("Hvs" with "[$]") as "[%|[H2 HT]]". *)
-(*   { iExFalso. iApply (ec_contradict with "[$]"). exact. } *)
-(*   iMod ("Hclose" with "[$Hε $H2 Htape H3 H4]") as "_". *)
-(*   { iNext. *)
-(*     iExists (<[α:=(ns ++ (nat_to_bool<$>(fin_to_nat <$> sample)))]>m). *)
-(*     rewrite fmap_insert. *)
-(*     rewrite big_sepM_insert_delete Heq/=. *)
-(*     rewrite fmap_delete. iFrame. *)
-(*     rewrite fmap_app/=. *)
-(*     rewrite !Hrewrite. iFrame. *)
-(*   } *)
-(*   iApply fupd_mask_intro_subseteq; first set_solver. *)
-(*   iFrame. rewrite fmap_app/=Hrewrite. iFrame. *)
-(*   erewrite (nnreal_ext _ _); first done. *)
-(*   simpl. by rewrite Nat.eqb_refl. *)
-(* Qed. *)
-
   
 End impl.
+
+
+(** * EXPERIMENT *)
+
+Class rand_spec' `{!conerisGS Σ} := RandSpec'
+{
+  (** * Operations *)
+  rand_allocate_tape' : val;
+  rand_tape' : val;
+  (** * Ghost state *)
+  (** The assumptions about [Σ] *)
+  randG' : gFunctors → Type;
+  
+  rand_tape_name': Type;
+  (** * Predicates *)
+  is_rand' {L : randG' Σ} (N:namespace)
+    (γ1: rand_tape_name') : iProp Σ;
+  rand_tapes_auth' {L : randG' Σ} (γ: rand_tape_name') (m:gmap loc (nat * list nat)): iProp Σ;
+  rand_tapes_frag' {L : randG' Σ} (γ: rand_tape_name') (α:loc) (ns: (nat * list nat)): iProp Σ;
+  (** * General properties of the predicates *)
+  #[global] is_rand_persistent' {L : randG' Σ} N γ1 ::
+    Persistent (is_rand' (L:=L) N γ1);
+  #[global] rand_tapes_auth_timeless' {L : randG' Σ} γ m ::
+    Timeless (rand_tapes_auth' (L:=L) γ m);
+  #[global] rand_tapes_frag_timeless' {L : randG' Σ} γ α ns ::
+    Timeless (rand_tapes_frag' (L:=L) γ α ns);
+  #[global] rand_tape_name_inhabited' ::
+    Inhabited rand_tape_name';
+
+  rand_tapes_auth_exclusive' {L : randG' Σ} γ m m':
+  rand_tapes_auth' (L:=L) γ m -∗ rand_tapes_auth' (L:=L) γ m' -∗ False;
+  rand_tapes_frag_exclusive' {L : randG' Σ} γ α ns ns':
+  rand_tapes_frag' (L:=L) γ α ns -∗ rand_tapes_frag' (L:=L) γ α ns' -∗ False;
+  rand_tapes_agree' {L : randG' Σ} γ α m ns:
+  rand_tapes_auth' (L:=L) γ m -∗ rand_tapes_frag' (L:=L) γ α ns -∗ ⌜ m!! α = Some (ns) ⌝;
+  rand_tapes_valid' {L : randG' Σ} γ2 α N E tb ns:
+    ⌜↑N⊆E⌝ ∗ is_rand' (L:=L) N γ2 ∗ rand_tapes_frag' (L:=L) γ2 α (tb, ns) ={E}=∗
+    ⌜Forall (λ n, n<=tb)%nat ns⌝;
+  rand_tapes_update' {L : randG' Σ} γ α m ns ns':
+    rand_tapes_auth' (L:=L) γ m -∗ rand_tapes_frag' (L:=L) γ α ns ==∗
+    rand_tapes_auth' (L:=L) γ (<[α := ns']> m) ∗ rand_tapes_frag' (L:=L) γ α ns';
+
+  (** * Program specs *)
+  rand_inv_create_spec' {L : randG' Σ} N E:
+  ⊢ wp_update E (∃ γ1, is_rand' (L:=L) N γ1);
+  rand_allocate_tape_spec' {L: randG' Σ} N E (tb:nat) γ2:
+    ↑N ⊆ E->
+    {{{ is_rand' (L:=L) N γ2 }}}
+      rand_allocate_tape' #tb @ E
+      {{{ (v:val), RET v;
+          ∃ (α:loc), ⌜v=#lbl:α⌝ ∗ rand_tapes_frag' (L:=L) γ2 α (tb, [])
+      }}};
+  rand_tape_spec_some' {L: randG' Σ} N E γ2 (P: iProp Σ) (Q:iProp Σ) (α:loc) (n:nat) (tb:nat) ns:
+    ↑N⊆E ->
+    {{{ is_rand' (L:=L) N γ2 ∗
+        □ (∀ (m:gmap loc (nat * list nat)), P ∗
+           rand_tapes_auth' (L:=L) γ2 m
+            ={E∖↑N}=∗ ⌜m!!α=Some (tb, n::ns)⌝ ∗ Q ∗ rand_tapes_auth' (L:=L) γ2 (<[α:=(tb, ns)]> m)) ∗
+        P
+    }}}
+      rand_tape' #lbl:α #tb @ E
+                       {{{ RET #n; Q }}};
+  rand_presample_spec' {L: randG' Σ} N E ns α (tb:nat)
+     (ε2 : list (fin (S tb)) -> R)
+    (P : iProp Σ) num T γ2 (ε:nonnegreal) :
+    ↑N ⊆ E ->
+    (∀ l, length l = num ->  0<= ε2 l)%R ->
+    (SeriesC (λ l, if bool_decide (l ∈ enum_uniform_fin_list tb num) then ε2 l else 0) /((S tb)^num) <= ε)%R->
+    is_rand' (L:=L) N γ2 -∗
+    □(∀ (ε': nonnegreal) m, P ∗ err_interp ε' ∗ rand_tapes_auth' (L:=L) γ2 m ={E∖↑N}=∗
+                   ⌜(ε<=ε')%R⌝ ∗ ⌜(m!!α = Some (tb, ns))⌝ ∗
+                   P ∗err_interp ε' ∗ rand_tapes_auth' (L:=L) γ2 m
+      ) -∗
+    (□∀ (ε': nonnegreal) ns' m, (P ∗ err_interp ε' ∗ ⌜length ns' = num⌝ ∗
+                     rand_tapes_auth' (L:=L) γ2 m
+                    ) ={E∖↑N}=∗
+                                (⌜(1<=ε2 ns' + (ε'-ε))%R⌝ ∨ ∃ (ε_final:nonnegreal),
+                                    ⌜(nonneg ε_final = ε2 ns' + (ε'-ε))%R ⌝ ∗
+                                    (err_interp ε_final ∗
+                                                       rand_tapes_auth' (L:=L) γ2 (<[α:= (tb, ns++(fin_to_nat <$> ns'))]> m) ∗ T ns')))
+        -∗
+    P -∗
+        wp_update E (∃ n, T n)
+}.
+
+Section impl'.
+  Local Opaque INR.
+  (* (** Instantiate rand *) *)
+  Class randG1' Σ := RandG1' { 
+                             flipG1_tapes':: hocap_tapesGS Σ;
+                      }.
+  Local Definition rand_inv_pred1' `{!conerisGS Σ, !hocap_tapesGS Σ} γ2:=
+    (∃ (m:gmap loc (nat * list nat)) ,
+        ([∗ map] α ↦ t ∈ m, α ↪N ( t.1 ; t.2 )) ∗
+        ●m@γ2
+    )%I.
+
+  #[local] Program Definition rand_spec1' `{!conerisGS Σ}: rand_spec' :=
+    {| rand_allocate_tape':= (λ: "N", alloc "N");
+      rand_tape':= (λ: "α" "N", rand("α") "N"); 
+      randG' := randG1';
+      rand_tape_name' := gname;
+      is_rand' _ N γ2 := inv N (rand_inv_pred1' γ2);
+      rand_tapes_auth' _ γ m := (●m@γ)%I;
+      rand_tapes_frag' _ γ α ns := (α ◯↪N (ns.1; ns.2) @ γ)%I;
+    |}.
+  Next Obligation.
+    simpl.
+    iIntros (??????) "H1 H2".
+    by iDestruct (ghost_map_auth_valid_2 with "[$][$]") as "[%H _]".
+  Qed.
+  Next Obligation.
+    simpl.
+    iIntros (???????) "H1 H2".
+    iDestruct (ghost_map_elem_frac_ne with "[$][$]") as "%"; last done.
+    rewrite dfrac_op_own dfrac_valid_own. by intro.
+  Qed.
+  Next Obligation.
+    simpl.
+    iIntros (??????[]) "??".
+    by iDestruct (hocap_tapes_agree with "[$][$]") as "%H".
+  Qed.
+  Next Obligation.
+    simpl.
+    iIntros (?????????) "(%&#Hinv&?)".
+    iInv "Hinv" as ">(%&?&?)" "Hclose".
+    iDestruct (hocap_tapes_agree with "[$][$]") as "%".
+    iDestruct (big_sepM_lookup_acc with "[$]") as "[H H']"; first done.
+    iDestruct (tapeN_ineq with "[$]") as "%".
+    iMod ("Hclose" with "[-]"); last done.
+    iFrame.
+    by iApply "H'".
+  Qed.
+  Next Obligation.
+    iIntros (???????[]) "??".
+    iMod (hocap_tapes_update with "[$][$]") as "[??]".
+    by iFrame.
+  Qed.
+  Next Obligation.
+    simpl.
+    iIntros (?????).
+    iApply fupd_wp_update_ret.
+    iMod (hocap_tapes_alloc ∅) as "(%γ2 & H4 & H5)".
+    iMod (inv_alloc _ _ (rand_inv_pred1' γ2) with "[-]").
+    { iFrame. by iNext. }
+    by iFrame.
+  Qed.
+  Next Obligation.
+    simpl.
+    iIntros (???????? Φ) "#Hinv HΦ".
+    wp_pures.
+    iInv "Hinv" as "(%&?&?)" "Hclose".
+    wp_apply (wp_alloc_tape); first done.
+    iIntros (α) "Hα".
+    iDestruct (hocap_tapes_notin with "[$][$]") as "%".
+    iMod (hocap_tapes_new _ _ α tb [] with "[$]") as "[?H]"; first done.
+    iMod ("Hclose" with "[-H HΦ]").
+    { iModIntro. iFrame.
+      rewrite big_sepM_insert; [iFrame|done].
+    }
+    iApply "HΦ".
+    by iFrame.
+  Qed.
+  Next Obligation.
+  simpl.
+  iIntros (????????????? Φ) "(#Hinv & #Hvs & HP) HΦ".
+  wp_pures.
+  wp_bind (rand(_) _)%E.
+  iInv "Hinv" as ">(%&H3&H4)" "Hclose".
+  iMod ("Hvs" with "[$]") as "(%&HQ&Hauth)".
+  iDestruct (big_sepM_insert_acc with "[$]") as "[Htape H3]"; first done.
+  simpl.
+  wp_apply (wp_rand_tape with "[$]") as "[Htape %]".
+  iMod ("Hclose" with "[- HΦ HQ]") as "_".
+  { iExists (<[α:=_]> m).
+    iFrame.
+    iApply "H3". by iNext.
+  }
+  by iApply "HΦ".
+Qed.
+Next Obligation.
+  simpl.
+  iIntros (?????????????? Hsubset Hpos Hineq) "#Hinv #Hcheck #Hvs HP ".
+  iApply wp_update_state_step_coupl.
+  iIntros (σ1 ε_supply) "((Hheap&Htapes)&Hε)".
+  iMod (inv_acc with "Hinv") as "[>(% & H3 & H4 ) Hclose]"; [done|].
+  iMod ("Hcheck" with "[$]") as "(%&%&HP&Hε& H4)".
+  iDestruct (big_sepM_insert_acc with "[$]") as "[Htape H3]"; first done.
+  simpl.
+  iDestruct (tapeN_lookup with "[$][$]") as "(%&%&%Heq)".
+  (* iDestruct (ec_supply_bound with "[$][$]") as "%". *)
+  (* iMod (ec_supply_decrease with "[$][$]") as (ε'' ε_rem -> Hε') "Hε_supply". subst. *)
+  iApply fupd_mask_intro; [set_solver|]; iIntros "Hclose'".
+  unshelve epose (ε_rem := mknonnegreal (ε_supply-ε) _).
+  { simpl in *. lra. }
+  replace (ε_supply) with (ε_rem + ε)%NNR; last first.
+  { rewrite /ε_rem. apply nnreal_ext. simpl. lra. }
+  iApply (state_step_coupl_iterM_state_adv_comp_con_prob_lang num α); first done.
+  unshelve iExists (λ x, mknonnegreal (if length x =? num then ε2 x else 1)%R _).
+  { case_match; last (simpl;lra). admit. }
+  iSplit.
+  { iPureIntro.
+    simpl. admit.
+    (* unshelve epose proof (Hineq ε1' _) as H'; first apply cond_nonneg. *)
+    (* etrans; last exact. *)
+    (* rewrite (Rdiv_def _ (2^_)) -SeriesC_scal_r. *)
+    (* etrans; last eapply (SeriesC_le_inj _ (λ x, Some (nat_to_bool <$> (fin_to_nat <$> x)))). *)
+    (* - apply SeriesC_le. *)
+    (*   + simpl. intros n. *)
+    (*     rewrite !fmap_length. *)
+    (*     case_match. *)
+    (*     * replace (1+1)%R with 2%R by lra. *)
+    (*       rewrite -Rdiv_1_l. simpl. *)
+    (*       split; last lra. *)
+    (*       apply Rmult_le_pos. *)
+    (*       -- apply Rcomplements.Rdiv_le_0_compat; first lra. *)
+    (*          apply pow_lt; lra. *)
+    (*       -- apply Hpos; first done. *)
+    (*          rewrite !fmap_length. *)
+    (*          by apply Nat.eqb_eq. *)
+    (*     * lra. *)
+    (*   + simpl. *)
+    (*     apply (ex_seriesC_list_length _ num). *)
+    (*     intros ?. rewrite !fmap_length. *)
+    (*     case_match; last lra. *)
+    (*     intros. by apply Nat.eqb_eq. *)
+    (* - intros. case_match; last lra. *)
+    (*   apply Rmult_le_pos; first apply Hpos; simpl; auto. *)
+    (*   + by apply Nat.eqb_eq. *)
+    (*   + rewrite -Rdiv_1_l. *)
+    (*     apply Rcomplements.Rdiv_le_0_compat; first lra. *)
+    (*     apply pow_lt; lra. *)
+    (* - intros ??? <- K. *)
+    (*   simplify_eq. *)
+    (*   rewrite -!list_fmap_compose in K. *)
+    (*   apply list_fmap_eq_inj in K; try done. *)
+    (*   intros x x'. *)
+    (*   repeat (inv_fin x; try intros x); *)
+    (*     repeat (inv_fin x'; try intros x'); done. *)
+    (* - apply (ex_seriesC_list_length _ num). *)
+    (*     intros ?. *)
+    (*     case_match; last lra. *)
+    (*     intros. by apply Nat.eqb_eq. *)
+  }
+  iIntros (sample) "<-".
+  destruct (Rlt_decision (nonneg ε_rem + (ε2 sample)%R) 1%R) as [Hdec|Hdec]; last first.
+  { apply Rnot_lt_ge, Rge_le in Hdec.
+    iApply state_step_coupl_ret_err_ge_1.
+    simpl. simpl in *. rewrite Nat.eqb_refl. lra.
+  }
+  iApply state_step_coupl_ret.
+  simpl.
+  rewrite -Heq.
+  iMod (tapeN_update_append' _ _ _ _ sample with "[$][$]") as "[Htapes Htape]".
+  iMod "Hclose'" as "_".
+  iMod ("Hvs" $! _ sample  with "[$HP $H4 $Hε]") as "Hor"; first done.  
+  iDestruct "Hor" as "[%|(%ε_final & %Heq' & Hε & Hauth & HT)]".
+  { exfalso. simpl in *. lra. }
+  iMod ("Hclose" with "[$Hauth Htape H3 ]") as "_".
+  { iNext.
+    by iApply "H3".
+  }
+  iApply fupd_mask_intro_subseteq; first set_solver.
+  iFrame. 
+  erewrite (nnreal_ext (_+_)%NNR _); first done.
+  simpl. rewrite Nat.eqb_refl. simpl in *. lra.
+Admitted.
+  
+End impl'.
 
